src/LeanEVM/FinVec.lean
@@ -1,0 +1,5 @@
+
+-- A set of zero or more bytes upto a given size.
+structure FinVec {n:Nat} (T) where
+  data : List T
+  isLt : data.length <= n
